More work from today and yesterday.  Weird problem with types in main body of the proof...

prf/ELF_Relocation_Proof.thy
@@ -11,17 +11,259 @@ imports
   "../auto_generated/isabelle/Test_image"
 begin
 
+section {* Proof-of-concept relocation proof *}
+
+subsection {* Useful definitions *}
+
+text {* Mov an immediate constant into a location in memory. *}
+definition mov_constant_to_mem :: "64 word \<Rightarrow> 64 word \<Rightarrow> instruction" where
+  "mov_constant_to_mem constant addr \<equiv> Zmov (Z_ALWAYS, (Z64, Zrm_i (Zm (None, (ZnoBase, addr)), constant)))"
+
+text {* Mov a constant from memory into the register RAX. *}
+definition mov_constant_from_mem :: "64 word \<Rightarrow> instruction" where
+  "mov_constant_from_mem addr \<equiv> Zmov (Z_ALWAYS, (Z64, Zr_rm (RAX, Zm (None, (ZnoBase, addr)))))"
+
+text {* The "fixed" program (i.e. the program that never changes and is never relocated) which
+moves the immediate constant 5 into a fixed address in memory and then moves that constant back into
+the RAX register using the two definitions above. *}
+definition fixed_program :: "8 word list" where
+  "fixed_program \<equiv>
+    List.concat (List.map encode [
+      mov_constant_to_mem (5 :: 64 word) (100 :: 64 word)
+    , mov_constant_from_mem (100 :: 64 word)
+    ])"
+
+text {* The program that will be relocated.  Moves an immediate constant 5 into some zero'd out
+address and will move the constant back again into the RAX register from the same address.  The zero'd
+out address will be "fixed-up" by the relocation process set up in Test_image.thy. *}
+definition relocatable_program :: "8 word list" where
+  "relocatable_program \<equiv>
+     List.concat (List.map encode [
+       mov_constant_to_mem (5 :: 64 word) (0 :: 64 word)
+     , mov_constant_from_mem (0 :: 64 word)
+     ])"
+
+text {* The relocation image that the linker produces internally after relocation.  The relocatable
+program above has now been relocated.  We will use this to populate a memory for the X64 emulation
+below. *}
+definition relocation_image :: "Abis.any_abi_feature annotated_memory_image" where
+  "relocation_image \<equiv> img1 relocatable_program"
+
+text {* Produce an X64 memory (a map from addresses to bytes) out of a memory image that we will
+obtain from the relocation_image above. *}
+definition X64_memory_of_memory_image :: "memory_image \<Rightarrow> (nat \<Rightarrow> 8 word)" where
+  "X64_memory_of_memory_image i addr =
+     (let keys = Map.dom i in
+      let rels = { s. \<forall>k \<in> keys. Some s = i k \<and> addr \<ge> the (startpos s) \<and> addr \<le> the (startpos s) + the (length1 s) } in
+      let arb  = Set.the_elem rels in
+      let reba = addr - the (startpos arb) in
+      let byte = List.nth (contents arb) reba in
+        the byte)"
+
+text {* Produces an initial state for the X64 emulation out of a memory_image (which will be converted
+to a memory, per the definition above) and a fixed start address for the instruction pointer.  This
+start address must match the start addresses of the .text section specified in Test_image.thy). *}
+definition load_relocated_program_image :: "memory_image \<Rightarrow> nat \<Rightarrow> X64_state" where
+  "load_relocated_program_image i entry_point \<equiv>
+     \<lparr> EFLAGS = \<lambda>x. None (* XXX: or False? *)
+     , MEM = \<lambda>a. X64_memory_of_memory_image i (unat a)
+     , REG = \<lambda>x. (0 :: 64 word)
+     , RIP = of_nat entry_point
+     , exception = NoException
+     \<rparr>"
+
+text {* Produces an initial state for the X64 emulation out of the encoded instructions of our fixed
+program above, and a fixed start address for the instruction pointer.  This start address must match
+the start address of the .text section specified in Test_image.thy. *}
+definition load_fixed_program_instructions :: "8 word list \<Rightarrow> nat \<Rightarrow> X64_state" where
+  "load_fixed_program_instructions p entry_point \<equiv>
+     \<lparr> EFLAGS = Map.empty (* XXX: or False? *)
+     , MEM = \<lambda>x. p ! (unat x - entry_point)
+     , REG = \<lambda>x. (0 :: 64 word)
+     , RIP = of_nat entry_point
+     , exception = NoException
+     \<rparr>"
+
+text {* Executes two steps of the X64 emulation given a fixed X64 state, returning a new state.  This
+will be sufficient to execute both programs above to their conclusion. *}
+definition run_two_steps :: "X64_state \<Rightarrow> X64_state" where
+  "run_two_steps \<sigma> \<equiv> snd (x64_next (snd (x64_next \<sigma>)))"
+
+text {* We now have our (rather silly) correctness property, which serves to demonstrate that our
+definitions are capable of supporting formal proof.  If we set the Isabelle execution mechanism up
+correctly we could just execute this to obtain our theorem, but we will use proof instead.  Creating
+two initial states for the X64 emulation out of our fixed and relocated program, we run them for two
+steps and demonstrate that the contents of their registers are the same after execution.  In
+particular, both RAX registers will contain the immediate constant, 5. *}
+definition correctness_property :: "bool" where
+  "correctness_property \<equiv>
+     let entry  = 4194304 in
+     let fstate1 = load_fixed_program_instructions fixed_program entry in
+     let fstate2 = run_two_steps fstate1 in
+     let rstate1 = load_relocated_program_image (elements relocation_image) entry in
+     let rstate2 = run_two_steps rstate1 in
+       REG rstate2 = REG rstate2 \<and> (REG rstate1) RAX = 5"
+
+subsection {* Lemmas *}
+
+lemma encode_relocated_program_compute:
+  shows "map encode [
+           Zmov (Z_ALWAYS, Z64, Zrm_i (Zm (None, ZnoBase, 0), 5)),
+           Zmov (Z_ALWAYS, Z64, Zr_rm (RAX, Zm (None, ZnoBase, 0)))
+         ] = [[72, 199, 4, 37, 0, 0, 0, 0, 5, 0, 0, 0], [72, 139, 4, 37, 0, 0, 0, 0]]"
+sorry (* XXX: true by eval *)
+
+lemma encode_fixed_program_compute:
+  shows "map encode [
+           Zmov (Z_ALWAYS, Z64, Zrm_i (Zm (None, ZnoBase, 100), 5)),
+           Zmov (Z_ALWAYS, Z64, Zr_rm (RAX, Zm (None, ZnoBase, 100)))
+         ] = [[72, 199, 4, 37, 100, 0, 0, 0, 5, 0, 0, 0], [72, 139, 4, 37, 100, 0, 0, 0]]"
+sorry (* XXX: true by eval *)
+
+lemma e_rm_imm_relocated_technical:
+  shows "List.concat [e_rm_imm (Z64, Zm (None, ZnoBase, 0), 5, 0, 198), e_rm_reg (Z64, Zm (None, ZnoBase, 0), word_of_int (int (Zreg_to_nat RAX)), [], 138)] =
+    [72, 199, 4, 37, 0, 0, 0, 0, 5, 0, 0, 0, 72, 139, 4, 37, 0, 0, 0, 0]"
+sorry (* XXX: true by eval *)
+
+lemma img1_technical:
+  shows "img1 [72, 199, 4, 37, 0, 0, 0, 0, 5, 0, 0, 0, 72, 139, 4, 37, 0, 0, 0, 0] = xxx"
+sorry
+
+(* XXX: ugly, but necessary to control the simplifier below *)
+lemma for_loop_19_unroll:
+  fixes act :: "nat \<Rightarrow> 'a \<Rightarrow> (unit \<times> 'a)"
+  shows "for_loop ((19::nat), 0, act) = (\<lambda>u. case act 19 u of
+     (u, ua) \<Rightarrow> case act 18 ua of
+                (u, ua) \<Rightarrow> case act 17 ua of
+                           (u, ua) \<Rightarrow> case act 16 ua of
+                                      (u, ua) \<Rightarrow> case act 15 ua of
+                                                 (u, ua) \<Rightarrow> case act 14 ua of
+                                                            (u, ua) \<Rightarrow> case act 13 ua of
+                                                                       (u, ua) \<Rightarrow> case act 12 ua of
+                                                                                  (u, ua) \<Rightarrow> case act 11 ua of
+                                                                                             (u, ua) \<Rightarrow> case act 10 ua of
+     (u, ua) \<Rightarrow> case act 9 ua of
+                (u, ua) \<Rightarrow> case act 8 ua of
+                           (u, ua) \<Rightarrow> case act 7 ua of
+                                      (u, ua) \<Rightarrow> case act 6 ua of
+                                                 (u, ua) \<Rightarrow> case act 5 ua of
+                                                            (u, ua) \<Rightarrow> case act 4 ua of (u, ua) \<Rightarrow> case act 3 ua of (u, ua) \<Rightarrow> case act 2 ua of (u, ua) \<Rightarrow> case act 1 ua of (u, x) \<Rightarrow> act 0 x)"
+  by simp
+
+(* XXX: need some precondition on size of x, here, but that's fine as we only ever use this lemma on
+   small constants...
+*)
+lemma word_arith_technical:
+  shows "unat (of_nat 4194304 + word_of_int (int x)) = (4194304 + x)"
+sorry
+
+lemma x64_fetch_fixed1:
+  shows "x64_fetch \<lparr>EFLAGS = Map.empty, MEM = \<lambda>x. [72, 199, 4, 37, 100, 0, 0, 0, 5, 0, 0, 0, 72, 139, 4, 37, 100, 0, 0, 0] ! (unat x - 4194304),
+                    REG = \<lambda>x. 0, RIP = of_nat 4194304, exception = NoException\<rparr> =
+          ([72, 199, 4, 37, 100, 0, 0, 0, 5, 0, 0, 0, 72, 139, 4, 37, 100, 0, 0, 0],
+           \<lparr>EFLAGS = Map.empty, MEM = \<lambda>x. [72, 199, 4, 37, 100, 0, 0, 0, 5, 0, 0, 0, 72, 139, 4, 37, 100, 0, 0, 0] ! (unat x - 4194304),
+            REG = \<lambda>x. 0, RIP = 4194304, exception = NoException\<rparr>)"
+apply(simp only: x64_fetch.simps for_loop_19_unroll)
+apply(simp only: snd_def split X64_state.simps fst_def)
+apply(simp only: word_arith_technical)
+apply simp
+done
+
+lemma x64_decode_fixed1:
+  shows "x64_decode [72, 199, 4, 37, 100, 0, 0, 0, 5, 0, 0, 0, 72, 139, 4, 37, 100, 0, 0, 0] =
+    Zfull_inst ([], Zmov (Z_ALWAYS, Z64, Zrm_i (Zm (None, ZnoBase, 100), 5)), [72, 139, 4, 37, 100, 0, 0, 0])"
+sorry (* XXX: true by eval *)
+
+lemma finite_maps_equal:
+  fixes f1 f2 :: "'a \<rightharpoonup> 'b"
+  assumes "\<forall>x \<in> dom f1 \<union> dom f2. f1 x = f2 x"
+  shows "f1 = f2"
+sorry
+
+declare [[show_types]]
+
+lemma Run_technical_fixed1:
+  shows "Run (Zmov (Z_ALWAYS, Z64, Zrm_i (Zm (None, ZnoBase, 100), 5)))
+     \<lparr>EFLAGS = Map.empty, MEM = \<lambda>x. [72, 199, 4, 37, 100, 0, 0, 0, 5, 0, 0, 0, 72, 139, 4, 37, 100, 0, 0, 0] ! (unat x - 4194304), REG = \<lambda>x. 0,
+        RIP = of_nat 4194304 + word_of_int (int (20 - length [72::8 word, 139, 4, 37, 100, 0, 0, 0])), exception = NoException\<rparr> =
+     ((), \<lparr>EFLAGS = Map.empty,
+            MEM = (\<lambda>x. [72, 199, 4, 37, 100, 0, 0, 0, 5, 0, 0, 0, 72, 139, 4, 37, 100, 0, 0, 0] ! (unat x - 4194304))
+              (100 := word_extract 7 0 (word_extract 15 0 (word_extract 31 0 (5::64 word))), 101 := word_extract 15 8 (word_extract 15 0 (word_extract 31 0 (5::64 word))),
+               102 := word_extract 7 0 (word_extract 31 16 (word_extract 31 0 (5::64 word))), 103 := word_extract 15 8 (word_extract 31 16 (word_extract 31 0 (5::64 word))),
+               104 := word_extract 7 0 (word_extract 15 0 (word_extract 63 32 (5::64 word))), 105 := word_extract 15 8 (word_extract 15 0 (word_extract 63 32 (5::64 word))),
+               106 := word_extract 7 0 (word_extract 31 16 (word_extract 63 32 (5::64 word))), 107 := word_extract 15 8 (word_extract 31 16 (word_extract 63 32 (5::64 word)))),
+            REG = \<lambda>x. 0, RIP = (of_nat 4194316)::64 word, exception = NoException\<rparr>)"
+  apply(simp only: Run.simps instruction.case dfn'Zmov.simps read_cond.simps Zcond.simps)
+  apply(simp only: Let_def split if_True fst_def EA.simps ea_Zsrc.simps Zdest_src.case)
+  apply(simp only: Zea.case restrictSize.simps Zsize.case split ea_Zdest.simps)
+  apply(simp only: Zdest_src.case split write'EA.simps fst_def ea_Zrm.simps Zrm.case ea_index.simps)
+  apply(simp only: option.case split Zea.case Zsize.case ea_base.simps Zbase.simps)
+  apply(simp only: write'mem64.simps write'mem32.simps write'mem16.simps write'mem8.simps)
+  apply(simp only: snd_def split X64_state.simps Pair_eq)
+  apply(rule conjI, simp only: refl; simp only: X64_state.ext_inject)
+  apply(simp only: refl simp_thms)
+  apply(rule conjI)
+  sorry (* XXX: weird problem with types, here *)
+
+declare [[show_types]]
+
+lemma x64_next_fixed1:
+  shows "x64_next \<lparr>EFLAGS = Map.empty,
+                                          MEM = \<lambda>x\<Colon>64 word. [72\<Colon>8 word, 199\<Colon>8 word, 4\<Colon>8 word, 37\<Colon>8 word, 100\<Colon>8 word, 0\<Colon>8 word, 0\<Colon>8 word, 0\<Colon>8 word, 5\<Colon>8 word, 0\<Colon>8 word, 0\<Colon>8 word, 0\<Colon>8 word, 72\<Colon>8 word,
+                                                             139\<Colon>8 word, 4\<Colon>8 word, 37\<Colon>8 word, 100\<Colon>8 word, 0\<Colon>8 word, 0\<Colon>8 word, 0\<Colon>8 word] !
+                                                            (unat x - (4194304\<Colon>nat)),
+                                          REG = \<lambda>x\<Colon>Zreg. 0\<Colon>64 word, RIP = of_nat (4194304\<Colon>nat), exception = NoException\<rparr> =
+         ((), \<lparr>EFLAGS = Map.empty,
+            MEM = (\<lambda>x. [72, 199, 4, 37, 100, 0, 0, 0, 5, 0, 0, 0, 72, 139, 4, 37, 100, 0, 0, 0] ! (unat x - 4194304))
+              (100 := word_extract 7 0 (word_extract 15 0 (word_extract 31 0 (5::64 word))), 101 := word_extract 15 8 (word_extract 15 0 (word_extract 31 0 (5::64 word))),
+               102 := word_extract 7 0 (word_extract 31 16 (word_extract 31 0 (5::64 word))), 103 := word_extract 15 8 (word_extract 31 16 (word_extract 31 0 (5::64 word))),
+               104 := word_extract 7 0 (word_extract 15 0 (word_extract 63 32 (5::64 word))), 105 := word_extract 15 8 (word_extract 15 0 (word_extract 63 32 (5::64 word))),
+               106 := word_extract 7 0 (word_extract 31 16 (word_extract 63 32 (5::64 word))), 107 := word_extract 15 8 (word_extract 31 16 (word_extract 63 32 (5::64 word)))),
+            REG = \<lambda>x. 0, RIP = of_nat 4194316, exception = NoException\<rparr>)"
+  apply(simp only: x64_next.simps x64_fetch_fixed1 fst_def split)
+  apply(simp only: x64_decode_fixed1 Zinst.case split X64_state.simps Run_technical_fixed1 word_arith_technical)
+done
+
+subsection {* The "big" theorem *}
+
+text {* Finally, our correctness theorem which shows that our correctness property holds: *}
+theorem correctness_property_True:
+  shows "correctness_property"
+unfolding correctness_property_def
+  (* Get rid of the entry address... *)
+  apply(subst Let_def)
+  (* Start working on the fixed program, first: *)
+  apply(simp only: fixed_program_def mov_constant_to_mem_def mov_constant_from_mem_def)
+  apply(simp only: encode_fixed_program_compute concat.simps append.simps)
+  apply(simp only: load_fixed_program_instructions_def)
+  (* Start running the two steps of the fixed program: *)
+  apply(subst Let_def)
+  apply(simp only: run_two_steps_def)
+(*
+  (* Start working on the relocated program, now: *)
+  apply(simp only: relocation_image_def relocatable_program_def mov_constant_to_mem_def mov_constant_from_mem_def)
+  apply(simp only: list.map encode.simps encode_relocated_program_compute)
+  apply(simp only: instruction.case split Zcond.case Zsize.case Zdest_src.case Zrm.case)
+  apply(simp only: e_rm_imm_relocated_technical)
+*)
+
+term Zm
+
+(*
+section {* OLD STUFF *}
+
 definition mov_constant_to_mem :: "64 word \<Rightarrow> 64 word \<Rightarrow> instruction" where
   "mov_constant_to_mem constant addr \<equiv> Zmov (Z_ALWAYS, (Z64, Zrm_i (Zm (None, (ZnoBase, addr)), constant)))"
 
 definition mov_constant_from_mem :: "64 word \<Rightarrow> instruction" where
   "mov_constant_from_mem addr \<equiv> Zmov (Z_ALWAYS, (Z64, Zr_rm (RAX, Zm (None, (ZnoBase, addr)))))"
 
-definition fixed_program :: "instruction list" where
+definition fixed_program :: "8 word list" where
   "fixed_program \<equiv>
-    [ mov_constant_to_mem (5 :: 64 word) (100 :: 64 word)
+    List.concat (List.map encode [
+      mov_constant_to_mem (5 :: 64 word) (100 :: 64 word)
     , mov_constant_from_mem (100 :: 64 word)
-    ]"
+    ])"
 
 definition relocatable_program :: "8 word list" where
   "relocatable_program \<equiv>
@@ -32,12 +274,6 @@ definition relocatable_program :: "8 word list" where
 
 definition relocation_image :: "Abis.any_abi_feature annotated_memory_image" where
   "relocation_image \<equiv> img1 relocatable_program"
-
-fun run_program :: "instruction list \<Rightarrow> X64_state \<Rightarrow> X64_state" where
-  "run_program [] \<sigma> = \<sigma>" |
-  "run_program (x#xs) \<sigma> =
-     (let (_, \<sigma>') = Run x \<sigma> in
-       run_program xs \<sigma>')"
 
 fun X64_memory_of_memory_image :: "memory_image \<Rightarrow> (nat \<Rightarrow> 8 word)" where
   "X64_memory_of_memory_image i addr =
@@ -52,6 +288,15 @@ definition load_image :: "memory_image \<Rightarrow> nat \<Rightarrow> X64_state
   "load_image i entry_point \<equiv>
      \<lparr> EFLAGS = \<lambda>x. None (* XXX: or False? *)
      , MEM = \<lambda>a. X64_memory_of_memory_image i (unat a)
+     , REG = \<lambda>x. (0 :: 64 word)
+     , RIP = of_nat entry_point
+     , exception = NoException
+     \<rparr>"
+
+definition load_program :: "8 word list \<Rightarrow> nat \<Rightarrow> X64_state" where
+  "load_program p entry_point \<equiv>
+     \<lparr> EFLAGS = Map.empty (* XXX: or False? *)
+     , MEM = \<lambda>x. p ! (unat x - entry_point)
      , REG = \<lambda>x. (0 :: 64 word)
      , RIP = of_nat entry_point
      , exception = NoException
@@ -73,34 +318,9 @@ definition execute_two_steps :: "X64_state \<Rightarrow> X64_state" where
               | _ \<Rightarrow> undefined))
        | _ \<Rightarrow> undefined))"
 
-definition initial_state :: "nat \<Rightarrow> X64_state" where
-  "initial_state entry \<equiv>
-    \<lparr> EFLAGS = \<lambda>x. None
-    , MEM = \<lambda>addr. 0
-    , REG = \<lambda>x. 0
-    , RIP = of_nat entry
-    , exception = NoException
-    \<rparr>"
-
 lemma let_ext:
-  shows "let (x, y) = z in q x y = q (fst z) (snd z)"
-by (cases z, auto)
-
-(* Theorem statement is something like:
- *
- * let ef = elf64_file_of_memory_image relocation_image in
- * let im = obtain_executable_image ef in
- * let \<sigma>0 = load_image im in
- *   run_program fixed_program empty_state \<simeq> execute_two_steps \<sigma>0
- *)
-
-definition relocation_test :: "nat \<Rightarrow> bool error" where
-  "relocation_test entry \<equiv>
-     (let i = elements relocation_image in
-      let rstate = load_image i entry in
-      let final_fixed_state = run_program fixed_program (initial_state entry) in
-      let final_relocatable_state = execute_two_steps rstate in
-        Success (REG final_fixed_state = REG final_relocatable_state))"
+  shows "let (x, y) = (u, v) in q x y = q u v"
+by auto
 
 lemma swap_pairs_lemma:
   shows "swap_pairs {(Some (''.text'', 1, 4), SymbolRef ref_and_reloc_rec0), (Some (''.data'', 0, 8), SymbolDef def_rec0)} =
@@ -108,6 +328,7 @@ lemma swap_pairs_lemma:
   apply(simp add: swap_pairs_def)
   apply auto
 done
+
 
 (* XXX: ugly, but necessary to control the simplifier below *)
 lemma for_loop_19_unroll:
@@ -132,9 +353,9 @@ lemma for_loop_19_unroll:
  
 lemma dom_lemma:
   shows "{a. [''.text'' \<mapsto>
-                      \<lparr>startpos = Some 4194304, length1 = Some 16,
+                      \<lparr>startpos = Some 4194304, length1 = Some 20,
                          contents = map Some (e_rm_imm (Z64, Zm (None, ZnoBase, 0), 5, 0, 198)) @ map Some (e_rm_reg (Z64, Zm (None, ZnoBase, 0), word_of_int (int (Zreg_to_nat RAX)), [], 138))\<rparr>,
-                      ''.data'' \<mapsto> \<lparr>startpos = Some 4194320, length1 = Some 8, contents = map Some (replicate 8 (of_nat 42))\<rparr>]
+                      ''.data'' \<mapsto> \<lparr>startpos = Some 4194324, length1 = Some 8, contents = map Some (replicate 8 (of_nat 42))\<rparr>]
                       a \<noteq>
                      None} = { ''.text'', ''.data''}"
   by auto
@@ -142,52 +363,112 @@ lemma dom_lemma:
 lemma rels_lemma:
   shows "{s. \<forall>k\<in>{''.text'', ''.data''}.
                         Some s = [''.text'' \<mapsto>
-                                  \<lparr>startpos = Some 4194304, length1 = Some 16,
+                                  \<lparr>startpos = Some 4194304, length1 = Some 20,
                                      contents = map Some (e_rm_imm (Z64, Zm (None, ZnoBase, 0), 5, 0, 198)) @
                                                 map Some (e_rm_reg (Z64, Zm (None, ZnoBase, 0), word_of_int (int (Zreg_to_nat RAX)), [], 138))\<rparr>,
-                                  ''.data'' \<mapsto> \<lparr>startpos = Some 4194320, length1 = Some 8, contents = map Some (replicate 8 (of_nat 42))\<rparr>]
+                                  ''.data'' \<mapsto> \<lparr>startpos = Some 4194324, length1 = Some 8, contents = map Some (replicate 8 (of_nat 42))\<rparr>]
                                   k \<and>
-                        the (startpos s) \<le> unat (of_nat 4194304 + word_of_int (int 0)) \<and> unat (of_nat 4194304 + word_of_int (int 0)) \<le> the (startpos s) + the (length1 s)} =
+                        the (startpos s) \<le> off \<and> off \<le> the (startpos s) + the (length1 s)} =
                                { \<lparr>startpos = Some 4194304, length1 = Some 16,
                                             contents = map Some (e_rm_imm (Z64, Zm (None, ZnoBase, 0), 5, 0, 198)) @
                                                        map Some (e_rm_reg (Z64, Zm (None, ZnoBase, 0), word_of_int (int (Zreg_to_nat RAX)), [], 138))\<rparr> }"
 sorry
 
 lemma the_elem_lemma:
-  shows "the_elem {\<lparr>startpos = Some 4194304, length1 = Some 16,
-                             contents = map Some (e_rm_imm (Z64, Zm (None, ZnoBase, 0), 5, 0, 198)) @
-                                        map Some (e_rm_reg (Z64, Zm (None, ZnoBase, 0), word_of_int (int (Zreg_to_nat RAX)), [], 138))\<rparr>} =
-                                        \<lparr>startpos = Some 4194304, length1 = Some 16,
-                             contents = map Some (e_rm_imm (Z64, Zm (None, ZnoBase, 0), 5, 0, 198)) @
-                                        map Some (e_rm_reg (Z64, Zm (None, ZnoBase, 0), word_of_int (int (Zreg_to_nat RAX)), [], 138))\<rparr>"
+  shows "the_elem { e } = e"
   by auto
 
 lemma word_calc_lemma:
-  shows "unat (of_nat 4194304 + word_of_int (int 0)) = 4194304"
+  shows "unat (of_nat 4194304 + word_of_int (int x)) = 4194304 + x"
 sorry
 
 lemma the_startpos_lemma:
-  shows "the (startpos \<lparr>startpos = Some 4194304, length1 = Some 16,
+  shows "the (startpos \<lparr>startpos = Some 4194304, length1 = Some 20,
                                   contents = map Some (e_rm_imm (Z64, Zm (None, ZnoBase, 0), 5, 0, 198)) @
                                              map Some (e_rm_reg (Z64, Zm (None, ZnoBase, 0), word_of_int (int (Zreg_to_nat RAX)), [], 138))\<rparr>) = 4194304"
   by auto
 
-lemma x64_fetch_lemma:
+lemma signed_arith_lemma1:
+  shows "(18446744071562067968 <=s 0 \<and> 0 <=s 2147483647) = True"
+sorry
+
+lemma signed_arith_lemma2:
+  shows "(18446744071562067968 <=s 5 \<and> 5 <=s 2147483647) = True"
+sorry
+
+lemma signed_arith_lemma3:
+  shows "(18446744071562067968 <=s 100 \<and> 100 <=s 2147483647) = True"
+sorry
+
+value "((word_cat (0::32 word) (word_cat ((word_extract 3 3 0)::16 word) (0::16 word)))::64 word) OR (8::64 word)"
+
+lemma word_cat_lemma:
+  shows "(word_cat 0 (word_cat (word_extract 3 3 0) 0) OR 8 = 0) = True"
+sorry
+
+lemma x64_fetch_lemma1:
   shows "x64_fetch \<lparr>EFLAGS = Map.empty,
-                       MEM = \<lambda>a\<Colon>64 word. X64_memory_of_memory_image
-                                          [''.text'' \<mapsto>
-                                           \<lparr>startpos = Some (4194304\<Colon>nat), length1 = Some (16\<Colon>nat),
-                                              contents = map Some (e_rm_imm (Z64, Zm (None, ZnoBase, 0\<Colon>64 word), 5\<Colon>64 word, 0\<Colon>4 word, 198\<Colon>8 word)) @
-                                                         map Some (e_rm_reg (Z64, Zm (None, ZnoBase, 0\<Colon>64 word), word_of_int (int (Zreg_to_nat RAX)), [], 138\<Colon>8 word))\<rparr>,
-                                           ''.data'' \<mapsto> \<lparr>startpos = Some (4194320\<Colon>nat), length1 = Some (8\<Colon>nat), contents = map Some (replicate (8\<Colon>nat) (of_nat (42\<Colon>nat)))\<rparr>]
-                                          (unat a),
-                       REG = \<lambda>x\<Colon>Zreg. 0\<Colon>64 word, RIP = of_nat (4194304\<Colon>nat), exception = NoException\<rparr> = xxx"
-  apply(simp only: x64_fetch.simps)
+                        MEM = \<lambda>a. X64_memory_of_memory_image
+                                   [''.text'' \<mapsto>
+                                    \<lparr>startpos = Some 4194304, length1 = Some 20,
+                                       contents = map Some (e_rm_imm (Z64, Zm (None, ZnoBase, 0), 5, 0, 198)) @
+                                                  map Some (e_rm_reg (Z64, Zm (None, ZnoBase, 0), word_of_int (int (Zreg_to_nat RAX)), [], 138))\<rparr>,
+                                    ''.data'' \<mapsto> \<lparr>startpos = Some 4194324, length1 = Some 8, contents = map Some (replicate 8 (of_nat 42))\<rparr>]
+                                   (unat a),
+                        REG = \<lambda>x. 0, RIP = of_nat 4194304, exception = NoException\<rparr> = ([72, 199, 4, 37, 0, 0, 0, 0, 5, 0, 0, 0], \<lparr>EFLAGS = Map.empty, MEM = \<lambda>a. the ([] ! (unat a - 4194304)), REG = \<lambda>x. 0, RIP = 4194316, exception = NoException\<rparr>)"
+sorry
+
+lemma x64_fetch_lemma2:
+  shows "x64_fetch (load_program fixed_program 4194304) = ([72, 199, 4, 37, 0, 0, 0, 0, 5, 0, 0, 0], \<lparr>EFLAGS = Map.empty, MEM = \<lambda>a. the ([] ! (unat a - 4194304)), REG = \<lambda>x. 0, RIP = 4194316, exception = NoException\<rparr>)"
+sorry
+
+value "x64_decode
+               (fst (snd (for_loop (19, 0, \<lambda>i state. ((), MEM (snd state) (RIP (snd state) + word_of_int (int i)) # fst state, snd state))
+                           ([], \<lparr>EFLAGS = Map.empty, MEM = \<lambda>x. fixed_program ! (unat x - 4194304), REG = \<lambda>x. 0, RIP = of_nat 4194304, exception = NoException\<rparr>))))"
+
+lemma x64_decode_lemma1:
+  shows "x64_decode
+               (fst (snd (for_loop (19, 0, \<lambda>i state. ((), MEM (snd state) (RIP (snd state) + word_of_int (int i)) # fst state, snd state))
+                           ([], \<lparr>EFLAGS = Map.empty, MEM = \<lambda>x. fixed_program ! (unat x - 4194304), REG = \<lambda>x. 0, RIP = of_nat 4194304, exception = NoException\<rparr>)))) = xxx"
+
+(*  apply(simp only: x64_fetch.simps)
   apply(simp only: Let_def)
   apply(simp only: for_loop_19_unroll)
   apply(simp only: split fst_def snd_def)
   apply(simp only: X64_state.simps)
   apply(simp only: X64_memory_of_memory_image.simps)
+
+  apply(simp only: dom_def; simp only: dom_lemma)
+
+  apply(subst Let_def; simp only: let_weak_cong[OF rels_lemma];
+          subst Let_def; simp only: the_elem_lemma; subst Let_def; simp only: element.simps option.sel word_calc_lemma;
+          subst Let_def; subst Let_def)+
+  apply(simp only: e_rm_reg.simps e_rm_imm.simps)
+  apply(simp only: e_ModRM.simps Zrm.case split option.case Zbase.case)
+  apply(simp only: e_imm32.simps)
+  apply(simp only: signed_arith_lemma1 if_True list.case split append.simps)
+  apply(simp only: e_opsize_imm.simps e_opsize.simps Zsize.case Let_def split)
+  apply(simp only: refl simp_thms if_True Zsize.case)
+  apply(simp only: e_imm32.simps signed_arith_lemma2 if_True list.case option.case split)
+  apply(simp only: concat.simps append.simps)
+  apply(simp only: rex_prefix.simps word_cat_lemma if_True append.simps list.map nth.simps)
+  apply simp
+(*
+  list.case split list.map append.simps)
+  apply(simp only: e_gen_rm_reg.simps)
+  apply(simp only: e_ModRM.simps Zrm.case split option.case Zbase.case)
+  apply(simp only: e_imm32.simps; simp only: signed_arith_lemma if_False list.case split list.map append.simps)
+  apply(simp)
+*)
+oops
+*)
+
+(*
+  apply(subst Let_def; simp only: let_weak_cong[OF rels_lemma];
+          subst Let_def; simp only: the_elem_lemma; subst Let_def; simp only: element.simps option.sel word_calc_lemma;
+          subst Let_def; subst Let_def)
+*)
+(*
   apply(simp only: dom_def)
   apply(simp only: dom_lemma)
   apply(subst Let_def)
@@ -196,13 +477,29 @@ lemma x64_fetch_lemma:
   apply(simp only: the_elem_lemma)
   apply(subst Let_def)
   apply(simp only: word_calc_lemma)
+  apply(simp only: the_startpos_lemma)
+  apply(subst Let_def)
+  apply(simp only: element.simps)
+  apply(subst diff_self_eq_0)
+  apply(subst Let_def)
+*)
+
+lemma x64_decode_lemma:
+  shows "x64_decode [72, 199, 4, 37, 0, 0, 0, 0, 5, 0, 0, 0] = Zfull_inst ([], Zmov (Z_ALWAYS, Z64, Zrm_i (Zm (None, ZnoBase, 0), 5)), [])"
+by eval
+
+lemma subst_hyp:
+  assumes "x = y" and "P x \<Longrightarrow> Q"
+  shows "P y \<Longrightarrow> Q"
+using assms by auto
 
 theorem at_least_some_relocations_relocate:
     fixes ef :: elf64_file and segs_and_provenance :: "(elf64_interpreted_segment \<times> segment_provenance) list" and entry :: "nat"
             and rstate final_fixed_state final_relocatable_state :: "X64_state"
   assumes "i = elements relocation_image" and "entry = 4194304"
       and "rstate = load_image i entry"
-      and "final_fixed_state = run_program fixed_program (initial_state entry)"
+      and "fstate = load_program fixed_program entry"
+      and "final_fixed_state = execute_two_steps fstate"
       and "final_relocatable_state = execute_two_steps rstate"
     shows "REG final_fixed_state = REG final_relocatable_state" (* XXX: probably want to say something about the contents of memory here, too! *)
 using assms
@@ -228,9 +525,25 @@ using assms
                           (SymbolRef null_symbol_reference_and_reloc_site) (tagEquiv instance_Abi_classes_AbiFeatureTagEquiv_Abis_any_abi_feature_dict)
                           {(SymbolRef ref_and_reloc_rec0, Some (''.text'', 1\<Colon>nat, 4\<Colon>nat)), (SymbolDef def_rec0, Some (''.data'', 0\<Colon>nat, 8\<Colon>nat))} None")
   apply(simp only: Let_def)
-  apply(simp only: option.case foldl.simps annotated_memory_image.simps)
+  apply(erule subst_hyp[where y ="None" and x="findLowestKVWithKEquivTo (instance_Basic_classes_Ord_Memory_image_range_tag_dict instance_Basic_classes_Ord_Abis_any_abi_feature_dict)
+                          (instance_Basic_classes_Ord_Maybe_maybe_dict
+                            (instance_Basic_classes_Ord_tup2_dict instance_Basic_classes_Ord_string_dict
+                              (instance_Basic_classes_Ord_tup2_dict instance_Basic_classes_Ord_Num_natural_dict instance_Basic_classes_Ord_Num_natural_dict)))
+                          (SymbolRef null_symbol_reference_and_reloc_site) (tagEquiv instance_Abi_classes_AbiFeatureTagEquiv_Abis_any_abi_feature_dict)
+                          {(SymbolRef ref_and_reloc_rec0, Some (''.text'', 1\<Colon>nat, 4\<Colon>nat)), (SymbolDef def_rec0, Some (''.data'', 0\<Colon>nat, 8\<Colon>nat))} None"])
+  apply(simp only: option.case foldl.simps annotated_memory_image.simps)+
   apply(simp only: execute_two_steps_def load_image_def)
-  apply(simp only: Let_def)
+  apply(simp only: x64_fetch_lemma1)
+  apply(simp only: Let_def split x64_decode_lemma Zinst.case)
+  apply(simp only: Run.simps instruction.case dfn'Zmov.simps read_cond.simps Zcond.case Let_def split)
+  apply(simp only: if_True ea_Zsrc.simps Zdest_src.case split fst_def EA.simps Zea.case)
+  apply(simp only: ea_Zdest.simps Zdest_src.case Zrm.case split fst_def ea_Zrm.simps ea_index.simps)
+  apply(simp only: option.case split ea_base.simps Zbase.case restrictSize.simps Zsize.case)
+  apply(simp only: write'EA.simps Zea.case split Zsize.case write'mem64.simps write'mem32.simps write'mem16.simps)
+  apply(simp only: write'mem8.simps snd_def split unit.case X64_state.simps add_0)
+  apply(simp only: load_program_def x64_fetch.simps Let_def split)
 
-
+thm restrictSize.simps
+term MEM
+*)
 end
